Common.v
@@ -1,3 +1,5 @@
 Global Set Implicit Arguments.
 Require Export Arith Omega List.
 Export ListNotations.
+
+Require Export StructTactics.
